Begin work adding better error-reporting/location-handling to PEGs

examples/formal-languages/context-free/locationScript.sml
@@ -2,22 +2,76 @@ open HolKernel Parse boolLib bossLib
 
 val _ = new_theory "location";
 
-val _ = Datatype `
- locn = <| row : num;  col : num; offset : num |>`;
+Datatype: locn = <| row : num;  col : num; offset : num |>
+End
 
-val _ = Datatype `
-  locs = Locs locn locn
-`
+Datatype: locs = Locs locn locn
+End
 
-val default_loc_def = Define`
-  default_loc = <| row := 1; col := 1; offset := 0 |>`;
+Definition default_loc_def:
+  default_loc = <| row := 1; col := 1; offset := 0 |>
+End
 
-val start_loc_def = Define`
-  start_loc = (default_loc,default_loc)`;
+Definition start_locs_def: start_locs = Locs default_loc default_loc
+End
 
-val unknown_loc_def = Define`
-  unknown_loc = Locs <| row := 0; col := 0; offset := 0 |>
-                     <| row := 0; col := 0; offset := 0 |>`;
+Definition end_locn_def:
+  end_locn = <| row := 0; col := 0; offset := 1 |>
+End
+
+Definition unknown_locn_def:
+  unknown_locn = <| row := 0; col := 0; offset := 0 |>
+End
+
+Definition unknown_loc_def:
+  unknown_loc = Locs unknown_locn unknown_locn
+End
+
+Definition locnle_def:
+  locnle l1 l2 <=>
+    l1 = l2 ∨ (* reflexivity, for free *)
+    l1 = default_loc ∨ (* minimal element *)
+    l2 = end_locn ∨ (* maximal element *)
+    (* otherwise compare row and col lexicographically*)
+    l1.row ≠ 0 ∧ l2.row ≠ 0 ∧ l1.col ≠ 0 ∧ l2.col ≠ 0 ∧
+    (l1.row < l2.row ∨ l1.row = l2.row ∧ l1.col < l2.col)
+End
+
+Theorem locn_rwts[simp]:
+  default_loc ≠ end_locn ∧ default_loc ≠ unknown_locn ∧
+  end_locn ≠ unknown_locn ∧ end_locn.row = 0 ∧
+  unknown_locn.row = 0 ∧ default_loc.row = 1 ∧ default_loc.col = 1
+Proof
+  simp[default_loc_def, end_locn_def, unknown_locn_def]
+QED
+
+Theorem locnle_REFL[simp]:
+  locnle loc loc
+Proof simp[locnle_def]
+QED
+
+Theorem locnle_TRANS:
+  locnle l1 l2 ∧ locnle l2 l3 ⇒ locnle l1 l3
+Proof
+  rw[locnle_def] >> fs[]
+QED
+
+Theorem locnle_end[simp]:
+  locnle end_locn l ⇔ l = end_locn
+Proof
+  simp[locnle_def]
+QED
+
+Theorem locnle_start[simp]:
+  locnle l default_loc ⇔ l = default_loc
+Proof
+  simp[locnle_def]
+QED
+
+Definition locsle_def:
+  locsle (Locs l1 _) (Locs l2 _) ⇔ locnle l1 l2
+End
+
 val merge_locs_def = Define`
   merge_locs (Locs l1 l2) (Locs l3 l4) = Locs l1 l4
 `;
