examples/formal-languages/context-free/pegScript.sml
@@ -11,60 +11,132 @@ val _ = new_theory "peg"
      DOI: 10.2168/LMCS-7(2:18)2011
 *)
 
-val _ = Hol_datatype `pegsym =
-    empty of 'c
-  | any of (('a # locs) -> 'c)
-  | tok of ('a -> bool) => (('a # locs) -> 'c)
-  | nt of 'b inf => ('c -> 'c)
-  | seq of pegsym => pegsym => ('c  -> 'c -> 'c)
-  | choice of pegsym => pegsym => ('c + 'c -> 'c)
-  | rpt of pegsym => ('c list -> 'c)
-  | not of pegsym => 'c
-`
+Datatype:
+  pegsym =
+    empty 'c
+  | any  (('a # locs) -> 'c)
+  | tok ('a -> bool) (('a # locs) -> 'c)
+  | nt ('b inf) ('c -> 'c)
+  | seq pegsym pegsym ('c  -> 'c -> 'c)
+  | choice pegsym pegsym ('c + 'c -> 'c)
+  | rpt pegsym ('c list -> 'c)
+  | not pegsym 'c
+  | error 'e
+End
 
-val _ = Hol_datatype`
-  peg = <| start : ('a,'b,'c) pegsym ;
-           rules : 'b inf |-> ('a,'b,'c) pegsym |>
-`
+Datatype:
+  peg = <| start : ('a,'b,'c,'e) pegsym ;
+           anyEOF : 'e ;
+           tokFALSE : 'e ; tokEOF : 'e;
+           notFAIL : 'e;
+           rules : 'b inf |-> ('a,'b,'c,'e) pegsym |>
+End
+
+Datatype:
+  pegresult = Success 'a 'c
+            | Failure locs 'e
+End
+Definition isSuccess_def[simp]:
+  isSuccess (Success _ _) = T ∧
+  isSuccess (Failure _ _) = F
+End
+Definition isFailure_def[simp]:
+  isFailure (Success _ _) = F ∧
+  isFailure (Failure _ _) = T
+End
+
+Definition resultmap_def[simp]:
+  resultmap f (Success a c) = Success a (f c) ∧
+  resultmap f (Failure fl fe) = Failure fl fe
+End
+Theorem resultmap_EQ_Success :
+  resultmap f r = Success a x ⇔ ∃x0. r = Success a x0 ∧ x = f x0
+Proof
+  Cases_on ‘r’ >> simp[] >> metis_tac[]
+QED
+
+Theorem resultmap_EQ_Failure[simp]:
+  (resultmap f r = Failure fl fe ⇔ r = Failure fl fe) ∧
+  (Failure fl fe = resultmap f r ⇔ r = Failure fl fe)
+Proof
+  Cases_on ‘r’ >> simp[] >> metis_tac[]
+QED
+Definition rmax_def[simp]:
+  rmax (Success a c) _ = Success a c ∧
+  rmax (Failure _ _) (Success a c) = Success a c ∧
+  rmax (Failure fl1 fe1) (Failure fl2 fe2) =
+  if locsle fl1 fl2 then Failure fl2 fe2 else Failure fl1 fe1
+End
+
+Theorem rmax_EQ_Success:
+  rmax r1 r2 = Success x y ⇔
+  r1 = Success x y ∨ r2 = Success x y ∧ isFailure r1
+Proof
+  Cases_on ‘r1’ >> simp[] >> Cases_on ‘r2’ >> simp[AllCaseEqs()]
+QED
+
+Theorem result_cases[local] = TypeBase.nchotomy_of “:(α,β,γ) pegresult”
+
+Definition sloc_def:
+  sloc [] = Locs end_locn end_locn ∧
+  sloc (h::t) = SND h
+End
+
+
 (* Option type should be replaced with sum type (loc. for NONE *)
 Inductive peg_eval:
-  (∀s c. peg_eval G (s, empty c) (SOME(s, c))) ∧
+  (∀s c. peg_eval G (s, empty c) (Success s c)) ∧
   (∀n r s f c.
-       n ∈ FDOM G.rules ∧ peg_eval G (s, G.rules ' n) (SOME(r,c)) ⇒
-       peg_eval G (s, nt n f) (SOME(r, f c))) ∧
-  (∀n s f.
-       n ∈ FDOM G.rules ∧ peg_eval G (s, G.rules ' n) NONE ⇒
-       peg_eval G (s, nt n f) NONE) ∧
-  (∀h t f. peg_eval G (h::t, any f) (SOME (t, f h))) ∧
-  (∀f. peg_eval G ([], any f) NONE) ∧
-  (∀e t P f. P (FST e) ⇒ peg_eval G (e::t, tok P f) (SOME(t, f e))) ∧
-  (∀e t P f. ¬P (FST e) ⇒ peg_eval G (e::t, tok P f) NONE) ∧
-  (∀P f. peg_eval G ([], tok P f) NONE) ∧
-  (∀e s c. peg_eval G (s, e) NONE ⇒ peg_eval G (s, not e c) (SOME(s,c))) ∧
-  (∀e s s' c. peg_eval G (s, e) (SOME s') ⇒ peg_eval G (s, not e c) NONE)  ∧
-  (∀e1 e2 s f. peg_eval G (s, e1) NONE ⇒ peg_eval G (s, seq e1 e2 f) NONE)  ∧
-  (∀e1 e2 s0 s1 c1 f.
-     peg_eval G (s0, e1) (SOME (s1, c1)) ∧ peg_eval G (s1, e2) NONE ⇒
-     peg_eval G (s0, seq e1 e2 f) NONE) ∧
+       n ∈ FDOM G.rules ∧ peg_eval G (s, G.rules ' n) (Success r c) ⇒
+       peg_eval G (s, nt n f) (Success r (f c))) ∧
+  (∀n s f fe fl.
+       n ∈ FDOM G.rules ∧ peg_eval G (s, G.rules ' n) (Failure fl fe) ⇒
+       peg_eval G (s, nt n f) (Failure fl fe)) ∧
+  (∀h t f. peg_eval G (h::t, any f) (Success t (f h))) ∧
+  (∀f. peg_eval G
+                ([] : ('a # locs) list, any f)
+                (Failure (sloc ([] : ('a # locs) list)) G.anyEOF)) ∧
+  (∀e t P f. P (FST e) ⇒ peg_eval G (e::t, tok P f) (Success t (f e))) ∧
+  (∀e t P f.
+     ¬P (FST e) ⇒
+     peg_eval G (e::t, tok P f) (Failure (sloc (e::t)) G.tokFALSE)) ∧
+  (∀P f. peg_eval G ([], tok P f)
+                  (Failure (sloc ([] : ('a # locs) list)) G.tokEOF)) ∧
+  (∀e s c fr.
+     peg_eval G (s, e) fr ∧ isFailure fr ⇒
+     peg_eval G (s, not e c) (Success s c)) ∧
+  (∀e s r c.
+     peg_eval G (s, e) r ∧ isSuccess r ⇒
+     peg_eval G (s, not e c) (Failure (sloc s) G.notFAIL))  ∧
+  (∀e1 e2 s f fr.
+     peg_eval G (s, e1) fr ∧ isFailure fr ⇒ peg_eval G (s, seq e1 e2 f) fr)  ∧
+  (∀e1 e2 s0 s1 c1 fr.
+     peg_eval G (s0, e1) (Success s1 c1) ∧
+     peg_eval G (s1, e2) fr ∧ isFailure fr ⇒
+     peg_eval G (s0, seq e1 e2 f) fr) ∧
   (∀e1 e2 s0 s1 s2 c1 c2 f.
-     peg_eval G (s0, e1) (SOME(s1, c1)) ∧
-     peg_eval G (s1, e2) (SOME(s2, c2)) ⇒
-     peg_eval G (s0, seq e1 e2 f) (SOME(s2, f c1 c2))) ∧
-  (∀e1 e2 s f.
-     peg_eval G (s, e1) NONE ∧ peg_eval G (s, e2) NONE ⇒
-     peg_eval G (s, choice e1 e2 f) NONE) ∧
-  (∀e1 e2 s s' f c.
-     peg_eval G (s, e1) (SOME(s',c)) ⇒
-     peg_eval G (s, choice e1 e2 f) (SOME(s', f (INL c)))) ∧
-  (∀e1 e2 s s' f c.
-     peg_eval G (s, e1) NONE ∧ peg_eval G (s, e2) (SOME(s',c)) ⇒
-     peg_eval G (s, choice e1 e2 f) (SOME(s',f (INR c))))  ∧
+     peg_eval G (s0, e1) (Success s1 c1) ∧
+     peg_eval G (s1, e2) (Success s2 c2) ⇒
+     peg_eval G (s0, seq e1 e2 f) (Success s2 (f c1 c2))) ∧
+  (∀e1 e2 s f f1 f2.
+     peg_eval G (s, e1) f1  ∧ peg_eval G (s, e2) f2 ∧
+     isFailure f1 ∧ isFailure f2 ⇒
+     peg_eval G (s, choice e1 e2 f) (rmax f1 f2)) ∧
+  (∀e1 e2 s f sr.
+     peg_eval G (s, e1) sr ∧ isSuccess sr ⇒
+     peg_eval G (s, choice e1 e2 f) (resultmap (f o INL) sr)) ∧
+  (∀e1 e2 s f fr sr.
+     peg_eval G (s, e1) fr ∧ isFailure fr ∧
+     peg_eval G (s, e2) sr ∧ isSuccess sr ⇒
+     peg_eval G (s, choice e1 e2 f) (resultmap (f o INR) sr)) ∧
+  (∀e s. peg_eval G (s, error e) (Failure (sloc s) e)) ∧
   (∀e f s s1 list.
      peg_eval_list G (s, e) (s1,list) ⇒
-     peg_eval G (s, rpt e f) (SOME(s1, f list))) ∧
-  (∀e s. peg_eval G (s, e) NONE ⇒ peg_eval_list G (s, e) (s,[])) ∧
+     peg_eval G (s, rpt e f) (Success s1 (f list))) ∧
+  (∀e s fr. peg_eval G (s, e) fr ∧ isFailure fr ⇒
+            peg_eval_list G (s, e) (s,[])) ∧
   (∀e s0 s1 s2 c cs.
-     peg_eval G (s0, e) (SOME(s1,c)) ∧
+     peg_eval G (s0, e) (Success s1 c) ∧
      peg_eval_list G (s1, e) (s2,cs) ⇒
      peg_eval_list G (s0, e) (s2,c::cs))
 End
@@ -77,36 +149,45 @@ Theorem peg_eval_strongind' =
     |> SIMP_RULE (srw_ss()) []
 
 open rich_listTheory
-val peg_eval_suffix0 = prove(
-  ``(∀s0 e sr. peg_eval G (s0,e) sr ⇒ ∀s r. sr = SOME (s,r) ⇒ IS_SUFFIX s0 s) ∧
-    ∀s0 e s rl. peg_eval_list G (s0,e) (s,rl) ⇒ IS_SUFFIX s0 s``,
+Theorem peg_eval_suffix0[local]:
+  (∀s0 e sr. peg_eval G (s0,e) sr ⇒ ∀s r. sr = Success s r ⇒ IS_SUFFIX s0 s) ∧
+  ∀s0 e s rl. peg_eval_list G (s0,e) (s,rl) ⇒ IS_SUFFIX s0 s
+Proof
   HO_MATCH_MP_TAC peg_eval_strongind' THEN
   SRW_TAC [][IS_SUFFIX_compute, IS_PREFIX_APPEND3, IS_PREFIX_REFL] THEN
-  METIS_TAC [IS_PREFIX_TRANS]);
+  fs[rmax_EQ_Success, resultmap_EQ_Success] >>
+  METIS_TAC [IS_PREFIX_TRANS]
+QED
 
 (* Theorem 3.1 *)
-val peg_eval_suffix = save_thm(
-  "peg_eval_suffix",
-  peg_eval_suffix0 |> SIMP_RULE (srw_ss() ++ DNF_ss) [])
+Theorem peg_eval_suffix =
+  peg_eval_suffix0 |> SIMP_RULE (srw_ss() ++ DNF_ss) []
 
 (* Theorem 3.2 *)
-val peg_deterministic = store_thm(
-  "peg_deterministic",
-  ``(∀s0 e sr. peg_eval G (s0,e) sr ⇒ ∀sr'. peg_eval G (s0,e) sr' ⇔ sr' = sr) ∧
-    ∀s0 e s rl. peg_eval_list G (s0,e) (s,rl) ⇒
-                ∀srl'. peg_eval_list G (s0,e) srl' ⇔ srl' = (s,rl)``,
+Theorem peg_deterministic:
+  (∀s0 e sr. peg_eval G (s0,e) sr ⇒ ∀sr'. peg_eval G (s0,e) sr' ⇔ sr' = sr) ∧
+  ∀s0 e s rl. peg_eval_list G (s0,e) (s,rl) ⇒
+              ∀srl'. peg_eval_list G (s0,e) srl' ⇔ srl' = (s,rl)
+Proof
   HO_MATCH_MP_TAC peg_eval_strongind' THEN SRW_TAC [][] THEN
-  ONCE_REWRITE_TAC [peg_eval_cases] THEN SRW_TAC [][]);
+  ONCE_REWRITE_TAC [peg_eval_cases] THEN SRW_TAC [][] THEN
+  TRY (Q.MATCH_ASSUM_RENAME_TAC ‘isSuccess result’ >>
+       Cases_on ‘result’ >> fs[]) THEN
+  TRY (Q.MATCH_ASSUM_RENAME_TAC ‘isFailure result’ >>
+       Cases_on ‘result’ >> fs[]) THEN csimp[] THEN
+  Q.MATCH_ASSUM_RENAME_TAC ‘isFailure result2’ >> Cases_on ‘result2’ >> fs[]
+QED
 
 (* Lemma 3.3 *)
-val peg_badrpt = store_thm(
-  "peg_badrpt",
-  ``peg_eval G (s0,e) (SOME(s0,r)) ⇒ ∀r. ¬peg_eval G (s0, rpt e f) r``,
+Theorem peg_badrpt:
+  peg_eval G (s0,e) (Success s0 r) ⇒ ∀r. ¬peg_eval G (s0, rpt e f) r
+Proof
   strip_tac >> simp[Once peg_eval_cases] >> map_every qx_gen_tac [`s1`, `l`] >>
   disch_then (assume_tac o MATCH_MP (CONJUNCT2 peg_deterministic)) >>
   `peg_eval_list G (s0,e) (s1,r::l)`
     by METIS_TAC [last (peg_eval_rules |> SPEC_ALL |> CONJUNCTS)] >>
-  pop_assum mp_tac >> simp[]);
+  pop_assum mp_tac >> simp[]
+QED
 
 Inductive peg0:
   (∀c. peg0 G (empty c)) ∧
@@ -149,49 +230,68 @@ Inductive peg0:
 
   (* not *)
   (∀e c. pegfail G e ⇒ peg0 G (not e c)) ∧
-  (∀e c. peg0 G e ∨ peggt0 G e ⇒ pegfail G (not e c))
+  (∀e c. peg0 G e ∨ peggt0 G e ⇒ pegfail G (not e c)) ∧
+
+  (* error *)
+  (∀e. pegfail G (error e))
 End
 
-val peg_eval_suffix' = store_thm(
-  "peg_eval_suffix'",
-  ``peg_eval G (s0,e) (SOME(s,c)) ⇒
-    s0 = s ∨ IS_SUFFIX s0 s ∧ LENGTH s < LENGTH s0``,
+Theorem peg_eval_suffix':
+  peg_eval G (s0,e) (Success s c) ⇒
+  s0 = s ∨ IS_SUFFIX s0 s ∧ LENGTH s < LENGTH s0
+Proof
   strip_tac >> imp_res_tac peg_eval_suffix >> Cases_on `s0 = s` >- simp[] >>
   fs[IS_SUFFIX_compute] >>
   imp_res_tac IS_PREFIX_LENGTH >> fs[] >>
   qsuff_tac `LENGTH s ≠ LENGTH s0` >- (strip_tac >> decide_tac) >>
   strip_tac >>
-  metis_tac [IS_PREFIX_LENGTH_ANTI, LENGTH_REVERSE, REVERSE_REVERSE]);
+  metis_tac [IS_PREFIX_LENGTH_ANTI, LENGTH_REVERSE, REVERSE_REVERSE]
+QED
 
-val peg_eval_list_suffix' = store_thm(
-  "peg_eval_list_suffix'",
-  ``peg_eval_list G (s0, e) (s,rl) ⇒
-    s0 = s ∨ IS_SUFFIX s0 s ∧ LENGTH s < LENGTH s0``,
+Theorem peg_eval_list_suffix':
+  peg_eval_list G (s0, e) (s,rl) ⇒
+  s0 = s ∨ IS_SUFFIX s0 s ∧ LENGTH s < LENGTH s0
+Proof
   strip_tac >> imp_res_tac peg_eval_suffix >> Cases_on `s0 = s` >- simp[] >>
   fs[IS_SUFFIX_compute] >> imp_res_tac IS_PREFIX_LENGTH >> fs[] >>
   qsuff_tac `LENGTH s ≠ LENGTH s0` >- (strip_tac >> decide_tac) >> strip_tac >>
-  metis_tac [IS_PREFIX_LENGTH_ANTI, LENGTH_REVERSE, REVERSE_REVERSE]);
-
+  metis_tac [IS_PREFIX_LENGTH_ANTI, LENGTH_REVERSE, REVERSE_REVERSE]
+QED
 
 fun rule_match th = FIRST (List.mapPartial (total MATCH_MP_TAC)
                                            (th |> SPEC_ALL |> CONJUNCTS))
 
-val lemma4_1a0 = prove(
-  ``(∀s0 e r. peg_eval G (s0, e) r ⇒
-              (∀c. r = SOME(s0,c) ⇒ peg0 G e) ∧
-              (r = NONE ⇒ pegfail G e) ∧
-              (∀s c. r = SOME(s,c) ∧ LENGTH s < LENGTH s0 ⇒ peggt0 G e)) ∧
-    (∀s0 e s rl. peg_eval_list G (s0,e) (s,rl) ⇒
-                 (s0 = s ⇒ pegfail G e) ∧
-                 (LENGTH s < LENGTH s0 ⇒ peggt0 G e))``,
-  ho_match_mp_tac peg_eval_strongind' >> simp[peg0_rules] >> rpt conj_tac
+Theorem FORALL_result:
+  (∀r. P r) ⇔ (∀a c. P (Success a c)) ∧ (∀fl fe. P (Failure fl fe))
+Proof
+  rw[EQ_IMP_THM] >> Cases_on ‘r’ >> simp[]
+QED
+
+Theorem EXISTS_result:
+  (∃r. P r) ⇔ (∃a c. P (Success a c)) ∨ (∃fl fe. P (Failure fl fe))
+Proof
+  rw[EQ_IMP_THM] >- (Cases_on ‘r’ >> metis_tac[]) >> metis_tac[]
+QED
+
+Theorem lemma4_1a0[local]:
+  (∀s0 e r. peg_eval G (s0, e) r ⇒
+            (∀c. r = Success s0 c ⇒ peg0 G e) ∧
+            (isFailure r ⇒ pegfail G e) ∧
+            (∀s c. r = Success s c ∧ LENGTH s < LENGTH s0 ⇒ peggt0 G e)) ∧
+  (∀s0 e s rl. peg_eval_list G (s0,e) (s,rl) ⇒
+               (s0 = s ⇒ pegfail G e) ∧
+               (LENGTH s < LENGTH s0 ⇒ peggt0 G e))
+Proof
+  ho_match_mp_tac peg_eval_strongind' >> simp[peg0_rules, FORALL_result] >>
+  rpt conj_tac
   >- (rpt strip_tac >> imp_res_tac peg_eval_suffix' >> fs[peg0_rules])
   >- (rpt strip_tac >> rule_match peg0_rules >>
       imp_res_tac peg_eval_suffix' >> fs[] >> rw[] >>
       full_simp_tac (srw_ss() ++ ARITH_ss) [])
   >- (rpt strip_tac >> rule_match peg0_rules >>
       imp_res_tac peg_eval_suffix' >> fs[] >> rw[] >>
-      full_simp_tac (srw_ss() ++ ARITH_ss) []) >>
+      full_simp_tac (srw_ss() ++ ARITH_ss) [])
+  >- simp[AllCaseEqs()] >>
   rpt strip_tac
   >- (first_x_assum match_mp_tac >> rw[] >>
       imp_res_tac peg_eval_suffix >> fs[IS_SUFFIX_compute] >>
@@ -200,15 +300,17 @@ val lemma4_1a0 = prove(
       metis_tac [IS_PREFIX_LENGTH_ANTI, LENGTH_REVERSE, REVERSE_REVERSE]) >>
   imp_res_tac peg_eval_suffix' >- rw[] >>
   imp_res_tac peg_eval_list_suffix' >- rw[] >>
-  asm_simp_tac (srw_ss() ++ ARITH_ss) [])
+  asm_simp_tac (srw_ss() ++ ARITH_ss) []
+QED
 
-val lemma4_1a = save_thm("lemma4_1a",lemma4_1a0 |> SIMP_RULE (srw_ss() ++ DNF_ss) [AND_IMP_INTRO])
+Theorem lemma4_1a = lemma4_1a0 |> SIMP_RULE (srw_ss() ++ DNF_ss) [AND_IMP_INTRO]
 
 Inductive wfpeg:
   (∀n f. n ∈ FDOM G.rules ∧ wfpeg G (G.rules ' n) ⇒ wfpeg G (nt n f)) ∧
   (∀c. wfpeg G (empty c)) ∧
   (∀f. wfpeg G (any f)) ∧
   (∀t f. wfpeg G (tok t f)) ∧
+  (∀e. wfpeg G (error e)) ∧
   (∀e c. wfpeg G e ⇒ wfpeg G (not e c)) ∧
   (∀e1 e2 f. wfpeg G e1 ∧ (peg0 G e1 ⇒ wfpeg G e2) ⇒
              wfpeg G (seq e1 e2 f)) ∧
@@ -220,6 +322,7 @@ Definition subexprs_def[simp]:
   (subexprs (any f1) = { any f1 }) ∧
   (subexprs (empty c) = { empty c }) ∧
   (subexprs (tok t f2) = { tok t f2 }) ∧
+  (subexprs (error e) = { error e }) ∧
   (subexprs (nt s f) = { nt s f }) ∧
   (subexprs (not e c) = not e c INSERT subexprs e) ∧
   (subexprs (seq e1 e2 f3) = seq e1 e2 f3 INSERT subexprs e1 ∪ subexprs e2) ∧
@@ -228,15 +331,13 @@ Definition subexprs_def[simp]:
   (subexprs (rpt e f5) = rpt e f5 INSERT subexprs e)
 End
 
+Theorem subexprs_included[simp]: e ∈ subexprs e
+Proof Induct_on `e` >> srw_tac[][subexprs_def]
+QED
 
-val subexprs_included = store_thm(
-  "subexprs_included",
-  ``e ∈ subexprs e``,
-  Induct_on `e` >> srw_tac[][subexprs_def] )
-
-val Gexprs_def = Define`
+Definition Gexprs_def:
   Gexprs G = BIGUNION (IMAGE subexprs (G.start INSERT FRANGE G.rules))
-`
+End
 
 Theorem start_IN_Gexprs[simp]:
   G.start ∈ Gexprs G
@@ -246,88 +347,105 @@ QED
 
 val wfG_def = Define`wfG G ⇔ ∀e. e ∈ Gexprs G ⇒ wfpeg G e`;
 
-val IN_subexprs_TRANS = store_thm(
-  "IN_subexprs_TRANS",
-  ``∀a b c. a ∈ subexprs b ∧ b ∈ subexprs c ⇒ a ∈ subexprs c``,
-  Induct_on `c` >> simp[] >> rpt strip_tac >> fs[] >> metis_tac[]);
+Theorem IN_subexprs_TRANS:
+  ∀a b c. a ∈ subexprs b ∧ b ∈ subexprs c ⇒ a ∈ subexprs c
+Proof
+  Induct_on `c` >> simp[] >> rpt strip_tac >> fs[] >> metis_tac[]
+QED
 
-val Gexprs_subexprs = store_thm(
-  "Gexprs_subexprs",
-  ``e ∈ Gexprs G ⇒ subexprs e ⊆ Gexprs G``,
+Theorem Gexprs_subexprs:
+  e ∈ Gexprs G ⇒ subexprs e ⊆ Gexprs G
+Proof
   simp_tac (srw_ss() ++ DNF_ss) [Gexprs_def, pred_setTheory.SUBSET_DEF] >>
-  strip_tac >> metis_tac [IN_subexprs_TRANS]);
+  strip_tac >> metis_tac [IN_subexprs_TRANS]
+QED
 
-val IN_Gexprs_E = store_thm(
-  "IN_Gexprs_E",
-  ``(not e c ∈ Gexprs G ⇒ e ∈ Gexprs G) ∧
-    (seq e1 e2 f ∈ Gexprs G ⇒ e1 ∈ Gexprs G ∧ e2 ∈ Gexprs G) ∧
-    (choice e1 e2 f2 ∈ Gexprs G ⇒ e1 ∈ Gexprs G ∧ e2 ∈ Gexprs G) ∧
-    (rpt e f3 ∈ Gexprs G ⇒ e ∈ Gexprs G)``,
+Theorem IN_Gexprs_E:
+  (not e c ∈ Gexprs G ⇒ e ∈ Gexprs G) ∧
+  (seq e1 e2 f ∈ Gexprs G ⇒ e1 ∈ Gexprs G ∧ e2 ∈ Gexprs G) ∧
+  (choice e1 e2 f2 ∈ Gexprs G ⇒ e1 ∈ Gexprs G ∧ e2 ∈ Gexprs G) ∧
+  (rpt e f3 ∈ Gexprs G ⇒ e ∈ Gexprs G)
+Proof
   rpt strip_tac >> imp_res_tac Gexprs_subexprs >> fs[] >>
-  metis_tac [pred_setTheory.SUBSET_DEF, subexprs_included]);
+  metis_tac [pred_setTheory.SUBSET_DEF, subexprs_included]
+QED
 
 val pair_CASES = pairTheory.pair_CASES
 val option_CASES = optionTheory.option_nchotomy
 val list_CASES = listTheory.list_CASES
 
-val reducing_peg_eval_makes_list = prove(
-  ``(∀s. LENGTH s < n ⇒ ∃r. peg_eval G (s, e) r) ∧ ¬peg0 G e ∧ LENGTH s0 < n ⇒
-    ∃s' rl. peg_eval_list G (s0,e) (s',rl)``,
+Theorem reducing_peg_eval_makes_list[local]:
+  (∀s. LENGTH s < n ⇒ ∃r. peg_eval G (s, e) r) ∧ ¬peg0 G e ∧ LENGTH s0 < n ⇒
+  ∃s' rl. peg_eval_list G (s0,e) (s',rl)
+Proof
   strip_tac >> completeInduct_on `LENGTH s0` >> rw[] >>
   full_simp_tac (srw_ss() ++ DNF_ss ++ ARITH_ss) [] >>
-  `peg_eval G (s0,e) NONE ∨ ∃s1 c. peg_eval G (s0,e) (SOME(s1,c))`
-    by metis_tac [pair_CASES, option_CASES]
-  >- metis_tac [peg_eval_rules] >>
+  ‘(∃fl fe. peg_eval G (s0,e) (Failure fl fe)) ∨
+   ∃s1 c. peg_eval G (s0,e) (Success s1 c)’
+    by metis_tac [result_cases]
+  >- metis_tac [peg_eval_rules,isFailure_def, isSuccess_def] >>
   `s0 ≠ s1` by metis_tac [lemma4_1a] >>
   `LENGTH s1 < LENGTH s0` by metis_tac [peg_eval_suffix'] >>
-  metis_tac [peg_eval_rules]);
+  metis_tac [peg_eval_rules]
+QED
 
-val peg_eval_total = store_thm(
-  "peg_eval_total",
-  ``wfG G ⇒ ∀s e. e ∈ Gexprs G ⇒ ∃r. peg_eval G (s,e) r``,
+Theorem peg_eval_total:
+  wfG G ⇒ ∀s e. e ∈ Gexprs G ⇒ ∃r. peg_eval G (s,e) r
+Proof
   simp[wfG_def] >> strip_tac >> gen_tac >>
-  completeInduct_on `LENGTH s` >>
+  completeInduct_on ‘LENGTH s’ >>
   full_simp_tac (srw_ss() ++ DNF_ss) [] >> rpt strip_tac >>
-  `wfpeg G e` by metis_tac[] >>
-  Q.UNDISCH_THEN `e ∈ Gexprs G` mp_tac >>
-  pop_assum mp_tac >> qid_spec_tac `e` >>
-  Induct_on `wfpeg` >> rw[]
+  ‘wfpeg G e’ by metis_tac[] >>
+  Q.UNDISCH_THEN ‘e ∈ Gexprs G’ mp_tac >>
+  pop_assum mp_tac >> qid_spec_tac ‘e’ >>
+  Induct_on ‘wfpeg’ >> rw[]
   >- ((* nt *)
-      qsuff_tac `G.rules ' n ∈ Gexprs G`
-      >- metis_tac [peg_eval_rules, option_CASES, pair_CASES] >>
+      qsuff_tac ‘G.rules ' n ∈ Gexprs G’
+      >- (strip_tac >>
+          first_x_assum $ drule_then
+                        $ qx_choose_then ‘result’ strip_assume_tac >>
+          Cases_on ‘result’ >>
+          metis_tac [peg_eval_rules]) >>
       asm_simp_tac (srw_ss() ++ DNF_ss) [Gexprs_def, FRANGE_DEF] >>
       metis_tac [subexprs_included])
   >- (* empty *) metis_tac [peg_eval_rules]
   >- (* any *) metis_tac [peg_eval_rules, list_CASES]
   >- (* tok *) metis_tac [peg_eval_rules, list_CASES]
-  >- (* not *) metis_tac [peg_eval_rules, optionTheory.option_nchotomy,
-                          IN_Gexprs_E]
-  >- ((* seq *) Q.MATCH_ASSUM_ABBREV_TAC `seq e1 e2 f ∈ Gexprs G` >>
-      markerLib.RM_ALL_ABBREVS_TAC >>
-      `e1 ∈ Gexprs G` by imp_res_tac IN_Gexprs_E >>
-      `peg_eval G (s,e1) NONE ∨ ∃s' c. peg_eval G (s,e1) (SOME(s',c))`
-        by metis_tac[option_CASES, pair_CASES]
-      >- metis_tac [peg_eval_rules] >>
-      Cases_on `s' = s`
-      >- (`peg0 G e1` by metis_tac [lemma4_1a] >>
-          `e2 ∈ Gexprs G` by imp_res_tac IN_Gexprs_E >>
-          metis_tac [peg_eval_rules, option_CASES, pair_CASES]) >>
-      `LENGTH s' < LENGTH s` by metis_tac [peg_eval_suffix'] >>
-      `∃r'. peg_eval G (s',e2) r'` by metis_tac [IN_Gexprs_E] >>
-      metis_tac [option_CASES, pair_CASES, peg_eval_rules])
+  >- (* error *) metis_tac[peg_eval_rules]
+  >- (* not *) metis_tac [peg_eval_rules, result_cases, IN_Gexprs_E,
+                          isSuccess_def, isFailure_def]
+  >- ((* seq *) rename [‘seq e1 e2 f ∈ Gexprs G’] >>
+      ‘e1 ∈ Gexprs G’ by imp_res_tac IN_Gexprs_E >>
+      ‘(∃fl fe. peg_eval G (s,e1) (Failure fl fe))  ∨
+       ∃s' c. peg_eval G (s,e1) (Success s' c)’
+        by metis_tac[result_cases]
+      >- metis_tac [peg_eval_rules, isFailure_def, isSuccess_def] >>
+      Cases_on ‘s' = s’
+      >- (‘peg0 G e1’ by metis_tac [lemma4_1a] >>
+          ‘e2 ∈ Gexprs G’ by imp_res_tac IN_Gexprs_E >>
+          metis_tac [peg_eval_rules, result_cases, isSuccess_def,
+                     isFailure_def]) >>
+      ‘LENGTH s' < LENGTH s’ by metis_tac [peg_eval_suffix'] >>
+      ‘∃r'. peg_eval G (s',e2) r'’ by metis_tac [IN_Gexprs_E] >>
+      metis_tac [result_cases, peg_eval_rules, isFailure_def, isSuccess_def])
   >- (* choice *)
-     metis_tac [peg_eval_rules, option_CASES, IN_Gexprs_E, pair_CASES] >>
+    (drule_then strip_assume_tac (cj 3 IN_Gexprs_E) >> fs[] >>
+     metis_tac [peg_eval_rules, result_cases, isSuccess_def, isFailure_def]) >>
   (* rpt *) imp_res_tac IN_Gexprs_E >>
-  `peg_eval G (s, e) NONE ∨ ∃s' c. peg_eval G (s,e) (SOME (s',c))`
-    by metis_tac [option_CASES, pair_CASES]
-  >- (`peg_eval_list G (s,e) (s,[])` by metis_tac [peg_eval_rules] >>
+  ‘(∃fl fe. peg_eval G (s, e) (Failure fl fe)) ∨
+   ∃s' c. peg_eval G (s,e) (Success s' c)’
+    by metis_tac [result_cases]
+  >- (‘peg_eval_list G (s,e) (s,[])’
+        by metis_tac [peg_eval_rules, isFailure_def] >>
       metis_tac [peg_eval_rules]) >>
-  `s' ≠ s` by metis_tac [lemma4_1a] >>
-  `LENGTH s' < LENGTH s` by metis_tac [peg_eval_suffix'] >>
-  metis_tac [peg_eval_rules, reducing_peg_eval_makes_list])
+  ‘s' ≠ s’ by metis_tac [lemma4_1a] >>
+  ‘LENGTH s' < LENGTH s’ by metis_tac [peg_eval_suffix'] >>
+  metis_tac [peg_eval_rules, reducing_peg_eval_makes_list]
+QED
 
 (* derived and useful PEG forms *)
-val pegf_def = Define`pegf sym f = seq sym (empty ARB) (λl1 l2. f l1)`
+Definition pegf_def:  pegf sym f = seq sym (empty ARB) (λl1 l2. f l1)
+End
 
 val ignoreL_def = Define`
   ignoreL s1 s2 = seq s1 s2 (λa b. b)
@@ -350,121 +468,135 @@ val checkAhead_def = Define`
   checkAhead P s = not (not (tok P ARB) ARB) ARB ~> s
 `;
 
-val peg_eval_seq_SOME = store_thm(
-  "peg_eval_seq_SOME",
-  ``peg_eval G (i0, seq s1 s2 f) (SOME (i,r)) ⇔
-    ∃i1 r1 r2. peg_eval G (i0, s1) (SOME (i1,r1)) ∧
-               peg_eval G (i1, s2) (SOME (i,r2)) ∧ (r = f r1 r2)``,
-  simp[Once peg_eval_cases] >> metis_tac[]);
+Theorem peg_eval_seq_SOME:
+  peg_eval G (i0, seq s1 s2 f) (Success i r) ⇔
+    ∃i1 r1 r2. peg_eval G (i0, s1) (Success i1 r1) ∧
+               peg_eval G (i1, s2) (Success i r2) ∧ (r = f r1 r2)
+Proof simp[Once peg_eval_cases] >> metis_tac[]
+QED
 
-val peg_eval_seq_NONE = store_thm(
-  "peg_eval_seq_NONE",
-  ``peg_eval G (i0, seq s1 s2 f) NONE ⇔
-      peg_eval G (i0, s1) NONE ∨
-      ∃i r. peg_eval G (i0,s1) (SOME(i,r)) ∧
-            peg_eval G (i,s2) NONE``,
-  simp[Once peg_eval_cases] >> metis_tac[]);
+Theorem peg_eval_seq_NONE:
+  peg_eval G (i0, seq s1 s2 f) (Failure fl fe) ⇔
+  peg_eval G (i0, s1) (Failure fl fe) ∨
+  ∃i r. peg_eval G (i0,s1) (Success i r) ∧
+        peg_eval G (i,s2) (Failure fl fe)
+Proof
+  simp[Once peg_eval_cases] >> metis_tac[]
+QED
 
-val peg_eval_tok_NONE = save_thm(
-  "peg_eval_tok_NONE",
-  ``peg_eval G (i, tok P f) NONE``
-    |> SIMP_CONV (srw_ss()) [Once peg_eval_cases])
+Theorem peg_eval_tok_NONE =
+  “peg_eval G (i, tok P f) (Failure fl fe)”
+    |> SIMP_CONV (srw_ss()) [Once peg_eval_cases]
 
-val peg_eval_tok_SOME = store_thm(
-  "peg_eval_tok_SOME",
-  ``peg_eval G (i0, tok P f) (SOME (i,r)) ⇔ ∃h. P (FST h) ∧ i0 = h::i ∧ r = f h``,
-  simp[Once peg_eval_cases] >> metis_tac[]);
+Theorem peg_eval_tok_SOME:
+  peg_eval G (i0, tok P f) (Success i r) ⇔
+  ∃h. P (FST h) ∧ i0 = h::i ∧ r = f h
+Proof simp[Once peg_eval_cases] >> metis_tac[]
+QED
 
-val peg_eval_empty = store_thm(
-  "peg_eval_empty[simp]",
-  ``peg_eval G (i, empty r) x ⇔ (x = SOME(i,r))``,
-  simp[Once peg_eval_cases])
+Theorem peg_eval_empty[simp]: peg_eval G (i, empty r) x ⇔ x = Success i r
+Proof simp[Once peg_eval_cases]
+QED
 
-val peg_eval_NT_SOME = store_thm(
-  "peg_eval_NT_SOME",
-  ``peg_eval G (i0,nt N f) (SOME(i,r)) ⇔
-      ∃r0. r = f r0 ∧ N ∈ FDOM G.rules ∧
-           peg_eval G (i0,G.rules ' N) (SOME(i,r0))``,
-  simp[Once peg_eval_cases]);
+Theorem peg_eval_NT_SOME:
+  peg_eval G (i0,nt N f) (Success i r) ⇔
+  ∃r0. r = f r0 ∧ N ∈ FDOM G.rules ∧
+       peg_eval G (i0,G.rules ' N) (Success i r0)
+Proof simp[Once peg_eval_cases]
+QED
 
-val peg_eval_choice = store_thm(
-  "peg_eval_choice",
-  ``∀x.
+Theorem peg_eval_choice:
+  ∀x.
      peg_eval G (i0, choice s1 s2 f) x ⇔
-      (∃i r. peg_eval G (i0, s1) (SOME(i, r)) ∧ x = SOME(i, f (INL r))) ∨
-      (∃i r. peg_eval G (i0, s1) NONE ∧
-             peg_eval G (i0, s2) (SOME(i, r)) ∧ x = SOME(i, f (INR r))) ∨
-      peg_eval G (i0, s1) NONE ∧ peg_eval G (i0,s2) NONE ∧ (x = NONE)``,
-  simp[Once peg_eval_cases, SimpLHS] >>
-  simp[optionTheory.FORALL_OPTION, pairTheory.FORALL_PROD] >> metis_tac[]);
+      (∃sr. peg_eval G (i0, s1) sr ∧ isSuccess sr ∧
+            x = resultmap (f o INL) sr) ∨
+      (∃sr fr.
+         peg_eval G (i0, s1) fr ∧ isFailure fr ∧
+         peg_eval G (i0, s2) sr ∧ isSuccess sr ∧ x = resultmap (f o INR) sr) ∨
+      ∃fr1 fr2.
+        peg_eval G (i0, s1) fr1 ∧ peg_eval G (i0, s2) fr2 ∧
+        isFailure fr1 ∧ isFailure fr2 ∧ x = rmax fr1 fr2
+Proof
+  simp[Once peg_eval_cases, SimpLHS] >> metis_tac[]
+QED
 
-val peg_eval_choicel_NIL = store_thm(
-  "peg_eval_choicel_NIL[simp]",
-  ``peg_eval G (i0, choicel []) x = (x = NONE)``,
-  simp[choicel_def, Once peg_eval_cases]);
+Theorem peg_eval_choicel_NIL[simp]:
+  peg_eval G (i0, choicel []) x = (x = Failure (sloc i0) G.notFAIL)
+Proof
+  simp[choicel_def, Once peg_eval_cases]
+QED
 
-val peg_eval_choicel_CONS = store_thm(
-  "peg_eval_choicel_CONS",
-  ``∀x. peg_eval G (i0, choicel (h::t)) x ⇔
-          peg_eval G (i0, h) x ∧ x <> NONE ∨
-          peg_eval G (i0,h) NONE ∧ peg_eval G (i0, choicel t) x``,
+Theorem peg_eval_choicel_CONS:
+  ∀x. peg_eval G (i0, choicel (h::t)) x ⇔
+      peg_eval G (i0, h) x ∧ isSuccess x ∨
+      ∃fr ry.
+        peg_eval G (i0,h) fr ∧ isFailure fr ∧ peg_eval G (i0, choicel t) ry ∧
+        x = rmax fr ry
+Proof
   simp[choicel_def, SimpLHS, Once peg_eval_cases] >>
-  simp[pairTheory.FORALL_PROD, optionTheory.FORALL_OPTION]);
+  dsimp[FORALL_result, resultmap_EQ_Success, rmax_EQ_Success] >>
+  conj_tac >- metis_tac[] >>
+  dsimp[EXISTS_result, AllCaseEqs()] >> metis_tac[]
+QED
 
-val peg_eval_rpt = store_thm(
-  "peg_eval_rpt",
-  ``peg_eval G (i0, rpt s f) x ⇔
-      ∃i l. peg_eval_list G (i0,s) (i,l) ∧ x = SOME(i,f l)``,
-  simp[Once peg_eval_cases, SimpLHS] >> metis_tac[]);
+Theorem peg_eval_rpt:
+  peg_eval G (i0, rpt s f) x ⇔
+      ∃i l. peg_eval_list G (i0,s) (i,l) ∧ x = Success i (f l)
+Proof simp[Once peg_eval_cases, SimpLHS] >> metis_tac[]
+QED
 
 val peg_eval_list = Q.store_thm(
   "peg_eval_list",
   `peg_eval_list G (i0, e) (i, r) ⇔
-     peg_eval G (i0, e) NONE ∧ i = i0 ∧ r = [] ∨
+     ∃fr. peg_eval G (i0, e) fr ∧ isFailure fr ∧ i = i0 ∧ r = [] ∨
      (∃i1 rh rt.
-        peg_eval G (i0, e) (SOME (i1, rh)) ∧
+        peg_eval G (i0, e) (Success i1 rh) ∧
         peg_eval_list G (i1, e) (i, rt) ∧ r = rh::rt)`,
   simp[Once peg_eval_cases, SimpLHS] >> metis_tac[]);
 
-val pegfail_empty = store_thm(
-  "pegfail_empty[simp]",
-  ``pegfail G (empty r) = F``,
-  simp[Once peg0_cases]);
+Theorem pegfail_empty[simp]:
+  pegfail G (empty r) = F
+Proof simp[Once peg0_cases]
+QED
 
-val peg0_empty = store_thm(
-  "peg0_empty[simp]",
-  ``peg0 G (empty r) = T``,
-  simp[Once peg0_cases]);
+Theorem peg0_empty[simp]:
+  peg0 G (empty r) = T
+Proof simp[Once peg0_cases]
+QED
 
-val peg0_not = store_thm(
-  "peg0_not[simp]",
-  ``peg0 G (not s r) ⇔ pegfail G s``,
-  simp[Once peg0_cases, SimpLHS]);
+Theorem peg0_not[simp]:
+  peg0 G (not s r) ⇔ pegfail G s
+Proof simp[Once peg0_cases, SimpLHS]
+QED
 
-val peg0_choice = store_thm(
-  "peg0_choice[simp]",
-  ``peg0 G (choice s1 s2 f) ⇔ peg0 G s1 ∨ pegfail G s1 ∧ peg0 G s2``,
-  simp[Once peg0_cases, SimpLHS]);
+Theorem peg0_choice[simp]:
+  peg0 G (choice s1 s2 f) ⇔ peg0 G s1 ∨ pegfail G s1 ∧ peg0 G s2
+Proof
+  simp[Once peg0_cases, SimpLHS]
+QED
 
-val peg0_choicel = store_thm(
-  "peg0_choicel[simp]",
-  ``(peg0 G (choicel []) = F) ∧
-    (peg0 G (choicel (h::t)) ⇔ peg0 G h ∨ pegfail G h ∧ peg0 G (choicel t))``,
-  simp[choicel_def])
+Theorem peg0_choicel[simp]:
+  (peg0 G (choicel []) = F) ∧
+  (peg0 G (choicel (h::t)) ⇔ peg0 G h ∨ pegfail G h ∧ peg0 G (choicel t))
+Proof
+  simp[choicel_def]
+QED
 
-val peg0_seq = store_thm(
-  "peg0_seq[simp]",
-  ``peg0 G (seq s1 s2 f) ⇔ peg0 G s1 ∧ peg0 G s2``,
-  simp[Once peg0_cases, SimpLHS])
+Theorem peg0_seq[simp]:
+  peg0 G (seq s1 s2 f) ⇔ peg0 G s1 ∧ peg0 G s2
+Proof simp[Once peg0_cases, SimpLHS]
+QED
 
-val peg0_tok = store_thm(
-  "peg0_tok[simp]",
-  ``peg0 G (tok P f) = F``,
-  simp[Once peg0_cases])
+Theorem peg0_tok[simp]:
+  peg0 G (tok P f) = F
+Proof
+  simp[Once peg0_cases]
+QED
 
-val peg0_pegf = store_thm(
-  "peg0_pegf[simp]",
-  ``peg0 G (pegf s f) = peg0 G s``,
-  simp[pegf_def])
+Theorem peg0_pegf[simp]:
+  peg0 G (pegf s f) = peg0 G s
+Proof
+  simp[pegf_def]
+QED
 
 val _ = export_theory()
